SlowTest/DiffLogic-Test/seq3_Dafny.dfy
@@ -1,3 +1,11 @@
+function method SeqUpdate<X> (s: seq<X>, k: int, v: X) : (s': seq<X>)
+    requires 0 <= k < |s|
+    ensures |s| == |s'|
+    ensures forall i :: 0 <= i < |s| ==>
+        if i < k then s'[i] == s[i]
+        else if i == k then s'[k] == v
+        else s'[i] == s[i]
+
 method Sequence(s: seq<bool>, j: int, b: bool, c: bool) returns (t: seq<bool>)
     requires 10 <= |s|
     requires 8 <= j < |s|
@@ -8,6 +16,7 @@ method Sequence(s: seq<bool>, j: int, b: bool, c: bool) returns (t: seq<bool>)
     if (c) {
       t := s[j := b];
     } else {
-      t := s[..j] + [b] + s[j+1..];
+        t := SeqUpdate<bool> (s, j, b);
+    //   t := s[..j] + [b] + s[j+1..];
     }
   }
